Hs/Examples/Sanity/HsCtx.lean
@@ -1,0 +1,2 @@
+import Hs.Examples.Sanity.HsCtx.Dnth
+import Hs.Examples.Sanity.HsCtx.Translate
