Hs/Examples/Sanity/HsCtx/Dnth.lean
@@ -1,0 +1,32 @@
+import Hs.HsTerm
+import Hs.HsCtx
+
+
+namespace HsCtx.dnth.Test
+
+def BF : HsFrame HsTerm :=
+   .datatypeDecl `★ [ `#0     -- Nothing :: ∀ a. Maybe a
+                    , `#1        -- , (`∀{`★} `#0 → `#3 `•k `#1)  -- Just :: ∀ a. a -> Maybe a
+                    ]
+
+
+def MBCtx : HsFrame HsTerm :=
+   .datatypeDecl (`★ `-k> `★) [ (`∀{`★} (`#1 `•k `#0))      -- Nothing :: ∀ a. Maybe a
+                              , (`∀{`★} `#0 → `#3 `•k `#1)  -- Just :: ∀ a. a -> Maybe a
+                              ]
+
+
+def ctx : HsCtx HsTerm := [MBCtx, BF]
+#eval ctx
+#eval ctx.length
+
+#eval (HsFrame.datatypeDecl `★ [ `#0 ]).width
+#eval [HsFrame.datatypeDecl `★ [ `#0 ]] d@s 0
+#eval [HsFrame.datatypeDecl `★ [ `#0 ]] d@s 1
+
+#eval [HsFrame.datatypeDecl `★ [ `#0, `#1 ]] d@s 0
+#eval [HsFrame.datatypeDecl `★ [ `#0, `#1 ]] d@s 1
+#eval [HsFrame.datatypeDecl `★ [ `#0, `#1 ]] d@s 2
+
+
+end HsCtx.dnth.Test
