Hs/Examples/Sanity/HsCtx/Translate.lean
@@ -1,0 +1,79 @@
+import Hs.Translator
+
+namespace HsCtx.Test.Translator
+
+def BF : HsFrame HsTerm :=
+   .datatypeDecl `★ [ `#0     -- Nothing :: ∀ a. Maybe a
+                    , `#1        -- , (`∀{`★} `#0 → `#3 `•k `#1)  -- Just :: ∀ a. a -> Maybe a
+                    ]
+
+
+def MBCtx : HsFrame HsTerm :=
+   .datatypeDecl (`★ `-k> `★) [ (`∀{`★} (`#1 `•k `#0))      -- Nothing :: ∀ a. Maybe a
+                              , (`∀{`★} `#0 → `#3 `•k `#1)  -- Just :: ∀ a. a -> Maybe a
+                              ]
+
+
+def ctx : HsCtx HsTerm := [MBCtx, BF]
+#eval ctx
+
+def ctx' := compile_ctx ctx
+
+@[simp]
+def check_compile_ctx_aux : HsCtx HsTerm -> DsM (List (FrameMetadata HsTerm × Frame Term)) := λ Γ => do
+  let Γ' <- compile_ctx Γ
+  return (List.map (λ i => (Γ s@ i, Γ' s@ i)) (Term.shift_helper (Γ'.length)))
+
+@[simp]
+def check_frame_equiv (Γ : Ctx Term) : FrameMetadata HsTerm -> Frame Term -> DsM Bool
+| .empty, .empty => return true
+| .tycon k, .datatype k' => do
+  let k'' <- compile_kind Γ □ k
+  return k'' == k'
+| .datacon τ, .ctor τ' => do
+  let τ'' <- compile_type Γ ★ τ
+  return τ'' == τ'
+| .type τ, .type τ' => do
+  let τ'' <- compile_type Γ ★ τ
+  return τ'' == τ'
+| _, _ => return false
+
+
+
+@[simp]
+def check_compile_ctx : HsCtx HsTerm -> DsM Bool := λ Γ => do
+  let ΓΓ' <- check_compile_ctx_aux Γ
+  let Γ' <- compile_ctx Γ
+  let x <- List.allM (λ x => check_frame_equiv Γ' x.1 x.2) ΓΓ'
+  return Γ'.length == Γ.length && x
+
+
+#eval DsM.run (check_compile_ctx_aux ((HsFrame.datatypeDecl `★ [`#0]) :: .nil))
+
+-- #eval DsM.run ctx'
+-- #eval ctx
+
+#eval DsM.run (check_compile_ctx_aux ctx)
+
+
+-- #eval DsM.run (check_compile_ctx_aux ((HsFrame.datatypeDecl `★ .nil) :: .nil))
+
+-- #eval DsM.run (check_compile_ctx_aux ((HsFrame.datatypeDecl `★ [`#0]) :: .nil))
+
+#guard check_compile_ctx ((HsFrame.datatypeDecl `★ .nil) :: .nil) == DsM.ok true
+
+
+-- #eval DsM.run (compile_ctx [HsFrame.datatypeDecl `★ [ `#0 ]])
+
+#guard check_compile_ctx ((HsFrame.datatypeDecl `★ [`#0]) :: .nil) == DsM.ok true
+
+#guard check_compile_ctx ctx == DsM.ok true
+
+
+-- #eval (ctx s@ 0)
+-- #eval DsM.run (do let c <- ctx'; return (c d@ 4))
+-- #eval (ctx s@ 4)
+
+
+
+end HsCtx.Test.Translator
