Hs/Utils.lean
@@ -1,0 +1,5 @@
+
+
+theorem List.reverse_length {l : List α}:
+  l.length = l.reverse.length := by
+induction l <;> simp at *
